theories/logic/compatibility.v
@@ -46,21 +46,22 @@ Section compatibility.
   Lemma sem_typed_unit Γ : 
     ⊢ Γ ⊨ #() : ⟨⟩ : () ⊨ Γ.
   Proof.
-    iIntros (vs) "!# HΓ₁ //=". iApply ewp_value. by iFrame.
+    iIntros (Φ vs) "!# HΓ₁ HΦ //=". iApply ewp_value. 
+    iApply "HΦ". by iFrame.
   Qed.
   
   Lemma sem_typed_bool Γ (b : bool) : 
     ⊢ Γ ⊨ #b : ⟨⟩ : 𝔹 ⊨ Γ.
   Proof.
-    iIntros (vs) "!# HΓ₁ //=". iApply ewp_value. 
-    iSplitR; first (iExists b); done.
+    iIntros (Φ vs) "!# HΓ₁ HΦ //=". iApply ewp_value. 
+    iApply "HΦ". iSplitR; first (iExists b); done.
   Qed.
   
   Lemma sem_typed_int Γ (i : Z) : 
     ⊢ Γ ⊨ #i : ⟨⟩ : ℤ ⊨ Γ.
   Proof.
-    iIntros (vs) "!# HΓ₁ //=". iApply ewp_value. 
-    iSplitR; first (iExists i); done.
+    iIntros (Φ vs) "!# HΓ₁ HΦ //=". iApply ewp_value. 
+    iApply "HΦ". iSplitR; first (iExists i); done.
   Qed.
   
   (* Subsumption rule *)
@@ -72,15 +73,14 @@ Section compatibility.
     τ'  ≤T τ →
     Γ₁' ⊨ e : ρ' : τ' ⊨ Γ₂' -∗ Γ₁ ⊨ e : ρ : τ ⊨ Γ₂.
   Proof.
-    iIntros (HΓ₁le HΓ₂le Hρle Hτle) "#He !# %vs HΓ₁ //=".
+    iIntros (HΓ₁le HΓ₂le Hρle Hτle) "#He !# %Φ %vs HΓ₁ HΦ //=".
     rewrite HΓ₁le.
     iApply ewp_os_prot_mono.
     { iApply Hρle. }
-    iApply (ewp_mono with "[HΓ₁ He]").
-    { by iApply "He". }
-    iIntros (v) "(Hτ' & HΓ₂)". iModIntro.
-    rewrite HΓ₂le.
-    iSplitR "HΓ₂"; first (iApply Hτle); done.
+    iApply ("He" with "HΓ₁").
+    iIntros (v) "[Hτ' HΓ₂]". iApply "HΦ".
+    rewrite HΓ₂le. iFrame.
+    by iApply Hτle.
   Qed. 
   
   (* λ-calculus rules *)
@@ -91,17 +91,17 @@ Section compatibility.
     (x,τ) :: Γ₁ ⊨ e : ρ : κ ⊨ [] -∗
     Γ₁ ++ Γ₂ ⊨ (λ: x, e) : ⟨⟩ : (τ -{ ρ }-∘ κ) ⊨ Γ₂.
   Proof.
-    iIntros (??) "#He !# %vs HΓ₁₂ //=".
+    iIntros (??) "#He !# %Φ %vs HΓ₁₂ HΦ //=".
     ewp_pure_steps. 
-    rewrite env_sem_typed_app. iDestruct "HΓ₁₂" as "[HΓ₁ $]".
-    iIntros (w) "Hτ". ewp_pure_steps.
+    rewrite env_sem_typed_app. iApply "HΦ". 
+    iDestruct "HΓ₁₂" as "[HΓ₁ $]".
+    iIntros (Φ' w) "Hτ HΦ'". ewp_pure_steps.
     rewrite -subst_map_insert. 
-    iApply (ewp_mono with "[HΓ₁ Hτ]").
-    - iApply "He". simpl. 
-      iSplitL "Hτ". 
-      { iExists w. iFrame. iPureIntro. apply lookup_insert. }
+    iApply ("He" with "[HΓ₁ Hτ] [HΦ']").
+    - iSplitL "Hτ". 
+      { iExists w. iIntros "{$Hτ} !%". apply lookup_insert. }
       by iApply env_sem_typed_insert.
-    - iIntros (v) "//= [Hκ _] !> {$Hκ}". 
+    - iIntros (v) "//= [Hκ _]". by iApply "HΦ'". 
   Qed.
   
   Lemma sem_typed_ufun Γ₁ Γ₂ f x e τ ρ κ: 
@@ -112,25 +112,26 @@ Section compatibility.
     (x,τ) :: (f, τ -{ ρ }-> κ) :: Γ₁ ⊨ e : ρ : κ ⊨ [] -∗
     Γ₁ ++ Γ₂ ⊨ (rec: f x := e) : ⟨⟩ : (τ -{ ρ }-> κ) ⊨ Γ₂.
   Proof.
-    iIntros (??? HcpyΓ₁) "#He !# %vs HΓ₁₂ //=".
+    iIntros (??? HcpyΓ₁) "#He !# %Φ %vs HΓ₁₂ HΦ //=".
     ewp_pure_steps.
-    rewrite env_sem_typed_app. iDestruct "HΓ₁₂" as "[HΓ₁ $]".
+    rewrite env_sem_typed_app. iApply "HΦ". 
+    iDestruct "HΓ₁₂" as "[HΓ₁ $]".
     rewrite HcpyΓ₁. iDestruct "HΓ₁" as "#HΓ₁".
     iLöb as "IH".
-    iIntros (w) "!# Hw". ewp_pure_steps. 
+    iIntros (Φ' w) "!# Hw HΦ'". ewp_pure_steps. 
     rewrite subst_subst_ne; last done.
     rewrite -subst_map_insert.
     rewrite -delete_insert_ne; last done. 
     rewrite -subst_map_insert.
-    iApply (ewp_mono with "[He Hw]").
-    - iApply "He". simpl in *. iSplitL "Hw"; last iSplitR "HΓ₁".
+    iApply ("He" with "[Hw] [HΦ']").
+    - iSplitL "Hw"; last iSplitR "HΓ₁".
       + iExists w. iFrame. iPureIntro.
         rewrite lookup_insert_ne; last done.
         by rewrite lookup_insert.
       + iExists _. iSplit; [by rewrite lookup_insert|]. 
         iApply "IH".
       + by do 2 (iApply env_sem_typed_insert; first done).
-    - iIntros (v) "(Hκ & _) !> {$Hκ}".
+    - iIntros (v) "[Hκ _]". by iApply "HΦ'". 
   Qed.
   
   Lemma sem_typed_app Γ₁ Γ₂ Γ₃ e₁ e₂ τ ρ κ: 
@@ -138,17 +139,15 @@ Section compatibility.
     Γ₁ ⊨ e₂ : ρ : τ ⊨ Γ₂ -∗
     Γ₁ ⊨ (e₁ e₂) : ρ : κ ⊨ Γ₃.
   Proof.
-    iIntros "#He₁ #He₂ !# %vs HΓ₁ //=".
+    iIntros "#He₁ #He₂ !# %Φ %vs HΓ₁ HΦ //=".
     iApply (ewp_bind ([AppRCtx (subst_map vs e₁)])); first done.
-    iApply (ewp_mono with "[HΓ₁]").
-    { by iApply "He₂". }
-    iIntros (v) "[Hτv HΓ₂] //= !>".
+    iApply ("He₂" with "HΓ₁").
+    iIntros (v) "[Hτ HΓ₂] //=".
     iApply (ewp_bind ([AppLCtx v])); first done.
-    iApply (ewp_mono with "[HΓ₂]").
-    { by iApply "He₁". }
-    iIntros (w) "[Hτκw HΓ₃] //= !>". 
-    iApply (ewp_frame_r with "[Hτκw Hτv] HΓ₃").
-    by iApply "Hτκw".
+    iApply ("He₁" with "HΓ₂").
+    iIntros (w) "[Hτκw HΓ₃] //=". 
+    iApply ("Hτκw" with "Hτ"). 
+    iIntros (u) "Hκ". iApply "HΦ". iFrame.
   Qed.
   
   Lemma sem_typed_pair Γ₁ Γ₂ Γ₃ e₁ e₂ τ ρ κ: 
@@ -156,16 +155,14 @@ Section compatibility.
     Γ₁ ⊨ e₂ : ρ : κ ⊨ Γ₂ -∗
     Γ₁ ⊨ (e₁,e₂) : ρ : (τ × κ) ⊨ Γ₃.
   Proof.
-    iIntros "#He₁ #He₂ !# %vs HΓ₁ //=".
+    iIntros "#He₁ #He₂ !# %Φ %vs HΓ₁ HΦ //=".
     iApply (ewp_bind ([PairRCtx (subst_map vs e₁)])); first done.
-    iApply (ewp_mono with "[HΓ₁]").
-    { by iApply "He₂". }
-    iIntros (v) "[Hτv HΓ₂] //= !>".
+    iApply ("He₂" with "HΓ₁").
+    iIntros (v) "[Hτv HΓ₂] //=".
     iApply (ewp_bind ([PairLCtx v])); first done.
-    iApply (ewp_mono with "[HΓ₂]").
-    { by iApply "He₁". }
-    iIntros (w) "[Hκw HΓ₃] //= !> ". ewp_pure_steps.
-    iFrame. iExists w, v. iFrame. by iPureIntro.
+    iApply ("He₁" with "HΓ₂").
+    iIntros (w) "[Hκw HΓ₃] //=". ewp_pure_steps.
+    iApply "HΦ". iFrame. iExists w, v. iFrame. by iPureIntro.
   Qed.
   
   Lemma sem_typed_pair_elim Γ₁ Γ₂ Γ₃ x₁ x₂ e₁ e₂ τ ρ κ ι: 
@@ -176,47 +173,92 @@ Section compatibility.
     (x₁, τ) :: (x₂, κ) :: Γ₂ ⊨ e₂ : ρ : ι ⊨ Γ₃ -∗
     Γ₁ ⊨ (let: (x₁, x₂) := e₁ in e₂) : ρ : ι ⊨ Γ₃.
   Proof.
-    iIntros (?????) "#He₁ #He₂ !# %vs HΓ₁ //=".
+    iIntros (?????) "#He₁ #He₂ !# %Φ %vs HΓ₁ HΦ //=".
     ewp_pure_steps.
     set ex1x2 := (λ: x₁ x₂, subst_map (binder_delete x₂ 
                                       (binder_delete x₁ vs)) e₂)%V. 
     iApply (ewp_bind ([AppLCtx ex1x2; AppRCtx pair_elim])); first done.
-    iApply (ewp_mono with "[HΓ₁]").
-    { by iApply "He₁". }
-    iIntros (v) "[Hτκv HΓ₂] !> //=". 
+    iApply ("He₁" with "HΓ₁").
+    iIntros (v) "[Hτκv HΓ₂] //=". 
     unfold pair_elim. ewp_pure_steps.
     iDestruct "Hτκv" as "(%v₁ & %v₂ & -> & Hτ & Hκ)".
     unfold ex1x2. ewp_pure_steps. 
     destruct (decide _) as [[]|[]]; [|split; [done|congruence]].
     rewrite delete_commute -subst_map_insert -delete_insert_ne; last congruence.
     rewrite <- subst_map_insert.
-    iApply (ewp_mono with "[Hτ Hκ HΓ₂]"). 
-    iApply "He₂". simpl. iSplitL "Hτ".
-    { iExists v₁. iFrame. iPureIntro. 
-      rewrite lookup_insert_ne; last done.
-      by rewrite lookup_insert. }
-    iSplitL "Hκ".
-    { iExists v₂. iFrame. iPureIntro. 
-      by rewrite lookup_insert. }
-    by repeat (iApply env_sem_typed_insert; first done).
-    iIntros (v) "[Hιv HΓ₃] !> {$Hιv}".
-    iApply (env_sem_typed_delete _ _ x₁ v₁); first done.
-    iApply (env_sem_typed_delete _ _ x₂ v₂); done.
+    iApply ("He₂" with "[Hτ Hκ HΓ₂]").
+    - iSplitL "Hτ".
+      { iExists v₁. iFrame. iPureIntro. 
+        rewrite lookup_insert_ne; last done.
+        by rewrite lookup_insert. }
+      iSplitL "Hκ".
+      { iExists v₂. iFrame. iPureIntro. 
+        by rewrite lookup_insert. }
+      by repeat (iApply env_sem_typed_insert; first done).
+    - iIntros (v) "[Hιv HΓ₃]". iApply "HΦ". iFrame.
+      iApply (env_sem_typed_delete _ _ x₁ v₁); first done.
+      iApply (env_sem_typed_delete _ _ x₂ v₂); done.
   Qed.
   
+  Lemma sem_typed_left_inj Γ₁ Γ₂ e τ ρ κ: 
+    Γ₁ ⊨ e : ρ : τ ⊨ Γ₂ -∗
+    Γ₁ ⊨ InjL e : ρ : (τ + κ) ⊨ Γ₂.
+  Proof.
+    iIntros "#He !# %Φ %vs HΓ₁ HΦ //=".
+    iApply (ewp_bind [InjLCtx]); first done.
+    iApply ("He" with "HΓ₁").
+    iIntros (v) "[Hv HΓ₂] //=".
+    ewp_pure_steps. iApply "HΦ".
+    iFrame. iExists v. iLeft. by iFrame.
+  Qed.
+
+  Lemma sem_typed_right_inj Γ₁ Γ₂ e τ ρ κ: 
+    Γ₁ ⊨ e : ρ : κ ⊨ Γ₂ -∗
+    Γ₁ ⊨ InjR e : ρ : (τ + κ) ⊨ Γ₂.
+  Proof.
+    iIntros "#He !# %Φ %vs HΓ₁ HΦ //=".
+    iApply (ewp_bind [InjRCtx]); first done.
+    iApply ("He" with "HΓ₁").
+    iIntros (v) "[Hv HΓ₂] //=".
+    ewp_pure_steps. iApply "HΦ".
+    iFrame. iExists v. iRight. by iFrame.
+  Qed.
+
+  Lemma sem_typed_case Γ₁ Γ₂ Γ₃ e₁ e₂ e₃ τ ρ κ ι: 
+    Γ₁ ⊨ e₁ : ρ : (τ + κ) ⊨ Γ₂ -∗
+    Γ₂ ⊨ e₂ : ⟨⟩ : (τ -{ ρ }-∘ ι) ⊨ Γ₃ -∗
+    Γ₂ ⊨ e₃ : ⟨⟩ : (κ -{ ρ }-∘ ι) ⊨ Γ₃ -∗
+    Γ₁ ⊨ Case e₁ e₂ e₃ : ρ : ι ⊨ Γ₃.
+  Proof.
+    iIntros "#He₁ #He₂ #He₃ !# %Φ %vs HΓ₁ HΦ //=".
+    iApply (ewp_bind [CaseCtx _ _]); first done.
+    iApply ("He₁" with "HΓ₁").
+    iIntros (v) "[(%w & [(-> & Hτ)|(-> & Hκ)]) HΓ₂] //="; 
+      ewp_pure_steps;
+      iApply (ewp_bind [AppLCtx _]); try done; 
+      ewp_bottom.
+    - iApply ("He₂" with "HΓ₂ [Hτ HΦ]").
+      iIntros (v) "[Hτι HΓ₃] //=".
+      iApply ("Hτι" with "Hτ"). 
+      iIntros (u) "Hι". iApply "HΦ". iFrame.
+    - iApply ("He₃" with "HΓ₂ [Hκ HΦ]").
+      iIntros (v) "[Hκι HΓ₃] //=".
+      iApply ("Hκι" with "Hκ"). 
+      iIntros (u) "Hκ". iApply "HΦ". iFrame.
+  Qed.
+
   Lemma sem_typed_un_op Γ₁ Γ₂ e op τ κ ρ: 
     typed_un_op op τ κ →
     Γ₁ ⊨ e : ρ : τ ⊨ Γ₂-∗
     Γ₁ ⊨ UnOp op e : ρ : κ ⊨ Γ₂.
   Proof.
-    iIntros (Hop) "#He !# %vs HΓ₁ //=".
+    iIntros (Hop) "#He !# %Φ %vs HΓ₁ HΦ //=".
     iApply (ewp_bind [UnOpCtx _]); first done.
-    iApply (ewp_mono with "[HΓ₁]").
-    { by iApply "He". }
-    iIntros (v) "[Hv HΓ₂] !> //=".
+    iApply ("He" with "HΓ₁").
+    iIntros (v) "[Hv HΓ₂] //=".
     destruct op; inversion_clear Hop;
-    iDestruct "Hv" as "(%n & ->)";
-    ewp_pure_steps; eauto.
+    iDestruct "Hv" as "(%n & ->)"; ewp_pure_steps; try done;
+    iApply "HΦ"; eauto.
   Qed.
   
   Lemma sem_typed_bin_op Γ₁ Γ₂ Γ₃ e₁ e₂ op τ κ ι ρ: 
@@ -225,19 +267,17 @@ Section compatibility.
     Γ₁ ⊨ e₂ : ρ : κ ⊨ Γ₂ -∗
     Γ₁ ⊨ BinOp op e₁ e₂ : ρ : ι ⊨ Γ₃.
   Proof.
-    iIntros (Hop) "#He₁ #He₂ !# %vs HΓ₁ //=".
+    iIntros (Hop) "#He₁ #He₂ !# %Φ %vs HΓ₁ HΦ //=".
     iApply (ewp_bind [BinOpRCtx _ _]); first done.
-    iApply (ewp_mono with "[HΓ₁]").
-    { by iApply "He₂". }
-    iIntros (v) "[Hv HΓ₂] !> //=". 
+    iApply ("He₂" with "HΓ₁").
+    iIntros (v) "[Hv HΓ₂] //=". 
     iApply (ewp_bind [BinOpLCtx _ _]); first done.
-    iApply (ewp_mono with "[HΓ₂]").
-    { by iApply "He₁". }
-    iIntros (w) "[Hw HΓ₃] !> //=". 
+    iApply ("He₁" with "HΓ₂").
+    iIntros (w) "[Hw HΓ₃] //=". 
     destruct op; inversion_clear Hop;
       iDestruct "Hv" as "(%n1 & ->)";
       iDestruct "Hw" as "(%n2 & ->)";
-      ewp_pure_steps; eauto.
+      ewp_pure_steps; try done; iApply "HΦ"; eauto.
   Qed.
   
   Lemma sem_typed_if Γ₁ Γ₂ Γ₃ e₁ e₂ e₃ ρ τ: 
@@ -246,14 +286,13 @@ Section compatibility.
     Γ₂ ⊨ e₃ : ρ : τ ⊨ Γ₃ -∗
     Γ₁ ⊨ (if: e₁ then e₂ else e₃) : ρ : τ ⊨ Γ₃.
   Proof.
-    iIntros "#He₁ #He₂ #He₃ !# %vs HΓ₁ //=".
+    iIntros "#He₁ #He₂ #He₃ !# %Φ %vs HΓ₁ HΦ //=".
     iApply (ewp_bind [IfCtx (subst_map vs e₂) (subst_map vs e₃)]) ;first done.
-    iApply (ewp_mono with "[HΓ₁]").
-    { by iApply "He₁". }
-    iIntros (v) "((%b & ->) & HΓ₃) !> //=".
+    iApply ("He₁" with "HΓ₁").
+    iIntros (v) "((%b & ->) & HΓ₂) //=".
     destruct b; ewp_pure_steps.
-    - by iApply "He₂".
-    - by iApply "He₃".
+    - iApply ("He₂" with "HΓ₂"). iFrame.
+    - iApply ("He₃" with "HΓ₂"). iFrame.
   Qed.
   
   (* Type abstraction and application *)
@@ -261,25 +300,26 @@ Section compatibility.
     (∀ A, Γ₁ ⊨ e : ρ : C A ⊨ []) -∗
     Γ₁ ++ Γ₂ ⊨ (Λ: e) : ⟨⟩ : (∀: A , ρ , C A)%T ⊨ Γ₂.
   Proof.
-    iIntros "#He !# %vs HΓ₁₂ //=".
+    iIntros "#He !# %Φ %vs HΓ₁₂ HΦ //=".
     rewrite env_sem_typed_app.
     iDestruct "HΓ₁₂" as "[HΓ₁ HΓ₂]".
-    ewp_pure_steps. iIntros "{$HΓ₂} %A //=". ewp_pure_steps.
-    iApply (ewp_mono with "[He HΓ₁]").
-    { by iApply "He". }
-    iIntros (w) "[HC _] !> {$HC}".
+    ewp_pure_steps. iApply "HΦ". 
+    iIntros "{$HΓ₂} %A //=". ewp_pure_steps.
+    iApply ("He" with "HΓ₁ []"). 
+    iIntros (w) "[HC _] {$HC}".
   Qed.
 
   Lemma sem_typed_TApp Γ₁ Γ₂ e ρ τ C : 
     Γ₁ ⊨ e : ρ : (∀: α , ρ , C α) ⊨ Γ₂ -∗
     Γ₁ ⊨ e <_> : ρ : C τ ⊨ Γ₂. 
   Proof.
-    iIntros "#He !# %vs HΓ₁ //=".
+    iIntros "#He !# %Φ %vs HΓ₁ HΦ //=".
     iApply (ewp_bind [AppLCtx _]); first done.
-    iApply (ewp_mono with "[HΓ₁]").
-    { by iApply "He". }
-    iIntros "%w [Hw HΓ₂] !> //=".
-    iApply (ewp_frame_r with "Hw HΓ₂").
+    iApply ("He" with "HΓ₁").
+    iIntros "%w [Hw HΓ₂] //=".
+    iApply (ewp_mono with "[Hw]").
+    { iApply "Hw". }
+    iIntros (u) "HC !>". iApply "HΦ". iFrame.
   Qed.
 
   (* Existential type packing and unpacking *)
@@ -287,12 +327,12 @@ Section compatibility.
     Γ₁ ⊨ e : ρ : C τ ⊨ Γ₂ -∗
     Γ₁ ⊨ (pack: e) : ρ : (∃: α, C α) ⊨ Γ₂. 
   Proof.
-    iIntros "#He %vs !# HΓ₁ //=".
+    iIntros "#He %Φ %vs !# HΓ₁ HΦ //=".
     iApply (ewp_bind [AppRCtx _]); first done.
-    iApply (ewp_mono with "[HΓ₁]"); [by iApply "He"|].
-    iIntros (v) "[Hτv HΓ₂] !> //=".
+    iApply ("He" with "HΓ₁").
+    iIntros (v) "[Hτv HΓ₂] //=".
     unfold exist_pack. ewp_pure_steps.
-    iFrame. by iExists τ. 
+    iApply "HΦ". iFrame. by iExists τ. 
   Qed.
 
   Lemma sem_typed_unpack Γ₁ Γ₂ Γ₃ x ρ e₁ e₂ κ C :
@@ -301,16 +341,16 @@ Section compatibility.
     (∀ τ, (x, C τ) :: Γ₂ ⊨ e₂ : ρ : κ ⊨ Γ₃) -∗
     Γ₁ ⊨ (unpack: x := e₁ in e₂) : ρ : κ ⊨ Γ₃.
   Proof.
-    iIntros (??) "#He₁ #He₂ %vs !# HΓ₁ //=".
+    iIntros (??) "#He₁ #He₂ %Φ %vs !# HΓ₁ HΦ //=".
     iApply (ewp_bind [AppRCtx _]); first done.
-    iApply (ewp_mono with "[HΓ₁]"); [by iApply "He₁"|].
-    iIntros (w) "[(%τ & Hτw) HΓ₂] !> //=". unfold exist_unpack.
+    iApply ("He₁" with "HΓ₁").
+    iIntros (w) "[(%τ & Hτw) HΓ₂] //=". unfold exist_unpack.
     ewp_pure_steps. rewrite -subst_map_insert.
-    iApply (ewp_mono with "[Hτw HΓ₂]").
-    - iApply "He₂". simpl. iSplitL "Hτw".
+    iApply ("He₂" with "[HΓ₂ Hτw]").
+    - simpl. iSplitL "Hτw".
       { iExists w. iFrame. iPureIntro. by rewrite lookup_insert. }
       by iApply env_sem_typed_insert.
-    - iIntros (u) "[Hκ HΓ₃] !> {$Hκ}".
+    - iIntros (u) "[Hκ HΓ₃]". iApply "HΦ". iFrame.
       by iApply env_sem_typed_delete.
   Qed.
 
@@ -319,11 +359,11 @@ Section compatibility.
     Γ₁ ⊨ e : ρ : (C (μ: α, C α)) ⊨ Γ₂ -∗
     Γ₁ ⊨ (fold: e) : ρ : (μ: α, C α) ⊨ Γ₂.
   Proof.
-    iIntros "#He %vs !# HΓ₁ //=".
+    iIntros "#He %Φ %vs !# HΓ₁ HΦ //=".
     iApply (ewp_bind [AppRCtx _]); first done. 
-    iApply (ewp_mono with "[HΓ₁]"); [by iApply "He"|].
-    iIntros "%w [HC HΓ₂] !> //=". 
-    unfold rec_fold. ewp_pure_steps.
+    iApply ("He" with "HΓ₁").
+    iIntros "%w [HC HΓ₂] //=". 
+    unfold rec_fold. ewp_pure_steps. iApply "HΦ".
     iFrame. by iApply sem_ty_rec_unfold. 
   Qed.
 
@@ -331,20 +371,21 @@ Section compatibility.
     Γ₁ ⊨ e : ρ : (μ: α, C α) ⊨ Γ₂ -∗
     Γ₁ ⊨ (unfold: e) : ρ : (C (μ: α, C α)) ⊨ Γ₂.
   Proof.
-    iIntros "#He %vs !# HΓ₁ //=".
+    iIntros "#He %Φ %vs !# HΓ₁ HΦ //=".
     iApply (ewp_bind [AppRCtx _]); first done. 
-    iApply (ewp_mono with "[HΓ₁]"); [by iApply "He"|].
-    iIntros "%w [Hμ HΓ₂] !> //=". 
+    iApply ("He" with "HΓ₁").
+    iIntros "%w [Hμ HΓ₂] //=". 
     rewrite sem_ty_rec_unfold. 
-    unfold rec_unfold. ewp_pure_steps. iFrame.
+    unfold rec_unfold. ewp_pure_steps. 
+    iApply "HΦ". iFrame.
   Qed.
 
   (* List type rules *)
   Lemma sem_typed_nil Γ τ: 
     ⊢ Γ ⊨ NIL : ⟨⟩ : List τ ⊨ Γ.
   Proof.
-    iIntros "!# %vs HΓ //=". 
-    ewp_pure_steps. unfold sem_ty_list.
+    iIntros "!# %Φ %vs HΓ HΦ //=". 
+    ewp_pure_steps. unfold sem_ty_list. iApply "HΦ".
     rewrite sem_ty_rec_unfold. iIntros "{$HΓ} !>".
     unfold ListF. iExists #(). by iLeft.
   Qed.
@@ -354,14 +395,14 @@ Section compatibility.
     Γ₁ ⊨ e₂ : ρ : List τ ⊨ Γ₂-∗
     Γ₁ ⊨ CONS e₁ e₂ : ρ : List τ ⊨ Γ₃.
   Proof.
-    iIntros "#He₁ #He₂ !# %vs HΓ₁ //=". 
+    iIntros "#He₁ #He₂ !# %Φ %vs HΓ₁ HΦ //=". 
     iApply (ewp_bind [InjRCtx; PairRCtx _]); first done.
-    iApply (ewp_mono with "[HΓ₁]").
-    { by iApply "He₂". }
-    iIntros (l) "[Hl HΓ₂] !> //=".
+    iApply ("He₂" with "HΓ₁").
+    iIntros (l) "[Hl HΓ₂] //=".
     iApply (ewp_bind [InjRCtx; PairLCtx _]); first done.
-    iApply (ewp_mono with "[HΓ₂]"); [by iApply "He₁"|].
-    iIntros (x) "[Hx HΓ₃] !> //=". ewp_pure_steps.
+    iApply ("He₁" with "HΓ₂").
+    iIntros (x) "[Hx HΓ₃] //=". ewp_pure_steps.
+    iApply "HΦ".
     unfold sem_ty_list. rewrite !sem_ty_rec_unfold.
     iIntros "{$HΓ₃} !>". iExists (x,l)%V. iRight. iSplit; first done.
     iExists x, l. iFrame; iSplit; first done.
@@ -380,13 +421,13 @@ Section compatibility.
           | NIL => e₂
          end : ρ : κ ⊨ Γ₃.
   Proof.
-    iIntros (?????) "#He₁ #He₂ #He₃ !# %vs HΓ₁ //=".
-    iApply (ewp_bind [CaseCtx _ _]); first done.
-    iApply (ewp_mono with "[HΓ₁]"); [by iApply sem_typed_unfold|simpl].
-    unfold sem_ty_list. iIntros (v₁) "[Hl HΓ₂] !>". ewp_pure_steps.
+    iIntros (?????) "#He₁ #He₂ #He₃ !# %Φ %vs HΓ₁ HΦ //=".
+    iApply (ewp_bind [CaseCtx _ _]); first done. 
+    iApply (sem_typed_unfold with "He₁ HΓ₁ [HΦ]"). simpl.
+    iIntros (v₁) "[Hl HΓ₂]". 
     iDestruct "Hl" as "(%v' & [[-> ->]|(-> & (%w₁ & %w₂ & -> & Hτ & Hμ))])"; 
     ewp_pure_steps.
-    { iApply ("He₂" with "[$HΓ₂]"). }
+    { iApply ("He₂" with "[$HΓ₂]"). iFrame. }
     rewrite lookup_delete. simpl.
     rewrite decide_False; [|by intros [_ []]].
     rewrite decide_True; last done. ewp_pure_steps.
@@ -396,9 +437,8 @@ Section compatibility.
     rewrite subst_subst_ne; [|congruence]. rewrite delete_commute.
     rewrite -subst_map_insert -delete_insert_ne; try congruence.
     rewrite -subst_map_insert. 
-    iApply (ewp_mono with "[Hτ Hμ HΓ₂]").
-    - iApply "He₃". simpl.
-      iSplitL "Hτ".
+    iApply ("He₃" with "[Hμ Hτ HΓ₂]").
+    - iSplitL "Hτ".
       { iExists w₁. iFrame. by rewrite lookup_insert. }
       iSplitL "Hμ".
       + iExists w₂. unfold sem_ty_list. iSplitR; [|done].
@@ -406,7 +446,7 @@ Section compatibility.
         by rewrite lookup_insert. 
       + iApply env_sem_typed_insert; first done.
         by iApply env_sem_typed_insert; first done.
-    - iIntros (u) "[Hκ HΓ₃] !> {$Hκ}".
+    - iIntros (u) "[Hκ HΓ₃]". iApply "HΦ". iFrame.
       iApply (env_sem_typed_delete _ _ xs w₂); first done.
       iApply (env_sem_typed_delete _ _ x w₁); done.
   Qed.
@@ -418,21 +458,20 @@ Section compatibility.
     Γ₁ ⊨ e : ρ : τ ⊨ Γ₂ -∗
     Γ₁ ⊨ ref e : ρ : Ref τ ⊨ Γ₂.
   Proof.
-    iIntros "#He !# %vs HΓ₁ //=".
+    iIntros "#He !# %Φ %vs HΓ₁ HΦ //=".
     iApply (ewp_bind [AllocCtx]); first done. simpl.
-    iApply (ewp_mono with "[HΓ₁]").
-    { by iApply "He". }
-    iIntros (v) "[Hτ HΓ₂] !>".
-    iApply ewp_alloc. iIntros "!> %l Hl !> {$HΓ₂}".
+    iApply ("He" with "HΓ₁").
+    iIntros (v) "[Hτ HΓ₂]".
+    iApply ewp_alloc. iIntros "!> %l Hl !>". iApply "HΦ". iFrame.
     iExists l. iSplit; first done. iExists v. iFrame.
   Qed.
   
   Lemma sem_typed_load Γ x ρ τ: 
     ⊢ ((x, Ref τ) :: Γ ⊨ !x : ρ : τ ⊨ (x, Ref Moved) :: Γ).
   Proof.
-    iIntros "%vs !# //= [(%v & -> & (%l & -> & (%w & Hl & Hτ))) HΓ] //=". 
+    iIntros "%Φ %vs !# //= [(%v & -> & (%l & -> & (%w & Hl & Hτ))) HΓ] HΦ //=". 
     iApply (ewp_load with "Hl").
-    iIntros "!> Hl !> {$Hτ} {$HΓ}". iExists #l.
+    iIntros "!> Hl !>". iApply "HΦ". iFrame. iExists #l.
     iSplitR; first done. iExists l. iSplitR; first done.
     iExists w. iFrame.
   Qed.
@@ -441,26 +480,24 @@ Section compatibility.
     copy_ty τ →
     ⊢ ((x, Ref τ) :: Γ ⊨ !x : ρ : τ ⊨ (x, Ref τ) :: Γ).
   Proof.
-    iIntros (Hcpy) "%vs !# //= [(%v & -> & (%l & -> & (%w & Hl & Hτ))) HΓ] //=". 
+    iIntros (Hcpy) "%Φ %vs !# //= [(%v & -> & (%l & -> & (%w & Hl & Hτ))) HΓ] HΦ //=". 
     iApply (ewp_load with "Hl").
-    unfold copy_ty, Persistent in Hcpy.
-    iDestruct (Hcpy w with "Hτ") as "#Hτ'". 
-    iIntros "!> Hl !> {$Hτ} {$HΓ}". iExists #l.
+    rewrite Hcpy. iDestruct "Hτ" as "#Hτ".
+    iIntros "!> Hl !>". iApply "HΦ". iIntros "{$Hτ $HΓ}". iExists #l.
     iSplitR; first done. iExists l. iSplitR; first done.
-    iExists w. iFrame. iApply "Hτ'".
+    iExists w. iIntros "{$Hτ $Hl}".
   Qed.
 
   Lemma sem_typed_store Γ₁ Γ₂ x e ρ τ κ: 
     Γ₁ ⊨ e : ρ : κ ⊨ Γ₂ -∗
     (x, Ref τ) :: Γ₁ ⊨ (x <- e) : ρ : () ⊨ (x, Ref κ) :: Γ₂.
   Proof.
-    iIntros "#He !# %vs //= [(%v & -> & (%l & -> & (%u & Hl & Hτ))) HΓ₁] //=".
+    iIntros "#He !# %Φ %vs //= [(%v & -> & (%l & -> & (%u & Hl & Hτ))) HΓ₁] HΦ //=".
     iApply (ewp_bind [StoreRCtx _]); first done. simpl.
-    iApply (ewp_mono with "[HΓ₁]").
-    { by iApply "He". }
-    iIntros (w) "[Hκ HΓ₂] !>".
-    iApply (ewp_store with "Hl"). iIntros "!> Hl !> {$HΓ₂}". 
-    iSplitR; first done. iExists #l. iSplitR; first done.
+    iApply ("He" with "HΓ₁").
+    iIntros (w) "[Hκ HΓ₂]". 
+    iApply (ewp_store with "Hl"). iIntros "!> Hl !>". iApply "HΦ". 
+    iFrame. iSplitR; first done. iExists #l. iSplitR; first done.
     iExists l. iSplitR; first done. iExists w. iFrame.
   Qed.
   
@@ -470,13 +507,13 @@ Section compatibility.
     Γ₁ ⊨ e : (ι ⇒ κ) : ι ⊨ Γ₂ -∗
     Γ₁ ⊨ (do: e) : (ι ⇒ κ) : κ ⊨ Γ₂.
   Proof.
-    iIntros "#He !# %vs HΓ₁ //=". 
+    iIntros "#He !# %Φ %vs HΓ₁ HΦ //=". 
     iApply (ewp_bind [DoCtx OS]); first done.
-    iApply (ewp_mono with "[HΓ₁]").
-    { by iApply "He". }
-    iIntros (v) "[Hι HΓ₂] !> //=".
+    iApply ("He" with "HΓ₁").
+    iIntros (v) "[Hι HΓ₂] //=".
     iApply ewp_do_os. rewrite upcl_sem_row_eff.
-    iExists v. eauto with iFrame.
+    iExists v. iFrame. iSplitR; first done.
+    iIntros (b) "Hκ". iApply "HΦ". iFrame.
   Qed.
   
 
@@ -499,37 +536,40 @@ Section compatibility.
     (x, τ') :: Γ₂ ++ Γ' ⊨ r x : ρ : τ ⊨ Γ₃ -∗
     Γ₁ ++ Γ' ⊨ (TryWith e (λ: w k, h w k) (λ: x, r x)) : (ι ⇒ κ) : τ ⊨ Γ₃.
   Proof.
-    iIntros (????????) "%ρ #He #Hh #Hr !# %vs HΓ₁' //=".
+    iIntros (????????) "%ρ #He #Hh #Hr !# %Φ %vs HΓ₁' HΦ //=".
     rewrite env_sem_typed_app. iDestruct "HΓ₁'" as "[HΓ₁ HΓ']".
     ewp_pure_steps.
-    iApply (ewp_try_with with "[HΓ₁]"); [by iApply "He"|].
+    iApply (ewp_try_with _ _ _ (λ v, τ' v ∗ env_sem_typed Γ₂ vs) 
+                    with "[HΓ₁] [HΓ' HΦ]"). 
+    { iApply ("He" with "HΓ₁"). iIntros "* [Hτ' HΓ₂] {$Hτ' $HΓ₂}". }
     iSplit; [|iSplit; iIntros (v c)];
     last (iIntros "?"; by rewrite upcl_bottom).
     - iIntros (v) "[Hv HΓ₂] //=". ewp_pure_steps.
       rewrite -subst_map_insert.
-      iApply (ewp_mono with "[HΓ₂ HΓ' Hv]").
-      + iApply "Hr". simpl. iSplitL "Hv".
+      iApply ("Hr" with "[HΓ₂ HΓ' Hv]").
+      + simpl. iSplitL "Hv".
         { iExists v. iIntros "{$Hv} !%". apply lookup_insert. }
         rewrite env_sem_typed_app. iFrame.
         iSplitL "HΓ₂"; by iApply env_sem_typed_insert.
-      + iIntros (u) "[Hw HΓ₃] !> //=".
-        iFrame. by iApply (env_sem_typed_delete _ _ x v).
+      + iIntros (u) "[Hw HΓ₃] //=".
+        iApply "HΦ". iFrame. by iApply (env_sem_typed_delete _ _ x v).
     - rewrite upcl_sem_row_eff.
       iIntros "(%a & -> & Ha & Hκb) //=". ewp_pure_steps.
       rewrite decide_True; [|split; first done; by injection].
       rewrite subst_subst_ne; last done.
       rewrite -subst_map_insert -delete_insert_ne; last done.
       rewrite -subst_map_insert.
-      iApply (ewp_mono with "[HΓ' Hκb Ha]").
-      + iApply "Hh". simpl. iSplitL "Ha".
+      iApply ("Hh" with "[HΓ' Hκb Ha]").
+      + simpl. iSplitL "Ha".
         { iExists a. iIntros "{$Ha} !%". apply lookup_insert. }
         iSplitL "Hκb".
         2: { do 2 (iApply env_sem_typed_insert; try done). }
         iExists c. iSplitR.
         { iPureIntro; rewrite lookup_insert_ne; last done; apply lookup_insert. }
-        iIntros (b) "Hb". iApply (ewp_mono with "[Hb Hκb]"); [by iApply "Hκb"|].
-        iIntros (?) "[? _] !> //=".
-      + iIntros (u) "[Hu HΓ₃] !> {$Hu}".
+        iIntros (Φ' b) "Hb HΦ'". 
+        iApply (ewp_mono with "[Hb Hκb]"); [by iApply "Hκb"|].
+        iIntros (?) "[? _] !> //=". by iApply "HΦ'".
+      + iIntros (u) "[Hu HΓ₃]". iApply "HΦ". iFrame.
         iApply (env_sem_typed_delete _ _ k c); first done.
         by iApply (env_sem_typed_delete _ _ w a).
   Qed.
@@ -544,25 +584,25 @@ Section compatibility.
     (x, τ) :: Γ₂ ++ Γ' ⊨ r x : ρ' : τ' ⊨ Γ₃ -∗
     Γ₁ ++ Γ' ⊨ (deep-try: e with effect (λ: w k, h w k) | return (λ: x, r x) end) : ρ' : τ' ⊨ Γ₃.
   Proof.
-    iIntros (???????? Hcpy) "%ρ #He #Hh #Hr !# %vs HΓ₁' //=".
-    rewrite env_sem_typed_app.
-    iDestruct "HΓ₁'" as "[HΓ₁ HΓ']".
-    unfold copy_env, Persistent in Hcpy.
-    iDestruct (Hcpy vs with "HΓ'") as "#HΓ".
-    ewp_pure_steps.
-    iApply (ewp_deep_try_with with "[HΓ₁]").
-    { by iApply "He". }
+    iIntros (???????? Hcpy) "%ρ #He #Hh #Hr !# %Φ %vs HΓ₁' HΦ //=".
+    rewrite env_sem_typed_app. iDestruct "HΓ₁'" as "[HΓ₁ HΓ']".
+    rewrite Hcpy. iDestruct "HΓ'" as "#HΓ'".
+    ewp_pure_steps. iApply (ewp_mono with "[HΓ₁] [HΦ]").
+    2: { simpl. iIntros "* H !>". iApply "HΦ". iApply "H". }
+    iApply (ewp_deep_try_with _ _ _ (λ v, τ v ∗ env_sem_typed Γ₂ vs) 
+                         with "[HΓ₁] []").
+    { iApply ("He" with "HΓ₁"). iIntros "* H {$H}". }
     iLöb as "IH". rewrite !deep_handler_unfold.
     iSplit; [|iSplit; iIntros (v c)];
     last (iIntros "?"; by rewrite upcl_bottom).
     - iIntros (v) "[Hv HΓ₂] //=". ewp_pure_steps.
-      rewrite -subst_map_insert. iApply (ewp_mono with "[Hv HΓ₂ HΓ']").
-      + iApply "Hr". simpl. iSplitL "Hv".
+      rewrite -subst_map_insert. 
+      iApply ("Hr" with "[Hv HΓ₂ HΓ']").
+      + simpl. iSplitL "Hv".
         iExists v. iIntros "{$Hv} !%". apply lookup_insert.
-        rewrite env_sem_typed_app. iSplitL "HΓ₂".
+        rewrite env_sem_typed_app. iSplitL "HΓ₂";
         by iApply env_sem_typed_insert.
-        by iApply env_sem_typed_insert.
-      + iIntros (?) "[Hτ' HΓ₃] !> {$Hτ'}".
+      + iIntros (?) "[Hτ' HΓ₃] {$Hτ'}".
         by iApply (env_sem_typed_delete _ _ x v).
     - rewrite upcl_sem_row_eff.
       iIntros "(%a & -> & Ha & Hκb)". ewp_pure_steps.
@@ -570,18 +610,17 @@ Section compatibility.
       rewrite subst_subst_ne; last done.
       rewrite -subst_map_insert -delete_insert_ne; last done.
       rewrite -subst_map_insert.
-      iApply (ewp_mono with "[Ha HΓ' Hκb]").
-      + iApply "Hh". simpl. iSplitL "Ha".
+      iApply ("Hh" with "[Ha HΓ' Hκb]").
+      + simpl. iSplitL "Ha".
         { iExists a; iIntros "{$Ha} !%"; apply lookup_insert. }
         iSplitL "Hκb".
         2: { do 2 (iApply env_sem_typed_insert; try done). }
         iExists c. iSplitR.
         { iPureIntro; rewrite lookup_insert_ne; last done; apply lookup_insert. }
-        iIntros (b) "Hb". iApply (ewp_mono with "[Hb Hκb]").
-        { iApply ("Hκb" with "Hb").
-          rewrite !deep_handler_unfold. iApply "IH". iApply "HΓ". }
-        iIntros (u) "[Hτ' HΓ₃] !> {$Hτ'}".
-      + iIntros (u) "[Hτ' HΓ₃] !> {$Hτ'}".
+        iIntros (Φ' b) "Hb HΦ'". iApply (ewp_mono with "[Hb Hκb] [HΦ']").
+        { iApply ("Hκb" with "Hb []"). rewrite !deep_handler_unfold. iApply "IH". }
+          iIntros "* [Hτ' HΓ₃] !>". by iApply "HΦ'".
+      + iIntros (u) "[Hτ' HΓ₃] {$Hτ'}".
         iApply (env_sem_typed_delete _ _ k c); first done.
         by iApply (env_sem_typed_delete _ _ w a).
     Qed.
